CertiGC/verif_forward.v
@@ -53,8 +53,8 @@ Proof.
     remember (graph_rep g * heap_rest_rep (ti_heap t_info) * outlier_rep outlier)
       as P. pose proof (graph_and_heap_rest_data_at_ _ _ _ H1 H).
     unfold generation_data_at_ in H12. remember (gen_start g from) as fp.
-    remember (nth_gen g from).(generation_sh) as fsh.
-    remember (gen_size t_info from) as gn. remember (WORD_SIZE * gn)%Z as fn.
+    remember (nth_sh g from) as fsh. remember (gen_size t_info from) as gn.
+    remember (WORD_SIZE * gn)%Z as fn.
     assert (P |-- (weak_derives P (memory_block fsh fn fp * TT) && emp) * P). {
       apply weak_derives_strong. subst. sep_apply H12.
       rewrite data_at__memory_block.
@@ -85,6 +85,7 @@ Proof.
         sep_apply (outlier_rep_single_rep _ _ _ H8 H4). Intros. gather_SEP 0 2.
         change (Vptr b i) with (GC_Pointer2val (GCPtr b i)) in v.
         pose proof (generation_share_writable (nth_gen g from)).
+        change (generation_sh (nth_gen g from)) with (nth_sh g from) in H13.
         rewrite <- Heqfsh in H13. unfold generation_data_at_.
         sep_apply (single_outlier_rep_memory_block_FF (GCPtr b i) fp gn fsh H13 v).
         assert_PROP False by entailer!. contradiction.
@@ -116,7 +117,10 @@ Proof.
       sep_apply (graph_and_heap_rest_v_in_range_iff _ _ _ _ H H1 H13). Intros.
       rewrite <- Heqfp, <- Heqgn, <- Heqfn in H14. destruct vv.
       * Intros. rewrite H14 in v0. clear H14. apply semax_if_seq. forward_if.
-        2: exfalso; inversion H14. admit.
+        2: exfalso; inversion H14. deadvars!. freeze [1; 2; 3; 4; 5; 6] FR.
+        localize [vertex_rep (nth_sh g (vgeneration v)) g v].
+        unlocalize [graph_rep g]. 1: apply (graph_vertex_ramif_stable _ _ H13).
+        admit.
       * apply semax_if_seq. forward_if. 1: exfalso; apply H15'; reflexivity.
         rewrite H14 in n. forward. rewrite <- Heqroot.
         Exists g t_info roots. simpl. entailer!.
